finished proofs + added ctx equivalence proofs for the sharded, linear and seq counters

theories/sharded_counter_modular.v
@@ -1,11 +1,12 @@
 From iris.algebra Require Import agree frac.
-From iris.base_logic.lib Require Import invariants.
+From iris.algebra.lib Require Import frac_auth.
+From iris.base_logic.lib Require Import ghost_map invariants mono_nat saved_prop.
 From iris.bi.lib Require Import fractional.
 From iris.heap_lang Require Import proofmode notation.
+From iris.heap_lang.lib Require Import par.
 From iris.prelude Require Import options.
 
 From summer_project Require Import counter_spec_modular.
-
 
 Definition msc_new_counter : val :=
   λ: "T", (AllocN "T" #0, "T").
@@ -25,84 +26,345 @@ Definition msc_sum_loop : val :=
 
 Definition msc_read : val :=
   λ: "c",
+    let: "p" := NewProph in
     let: "a" := Fst "c" in
     let: "T" := Snd "c" in
-    msc_sum_loop "a" "T" #0 #0.
+    let: "r" := msc_sum_loop "a" "T" #0 #0 in
+    ResolveProph "p" "r";;
+    "r".
 
-Definition msc_modelR : cmra := prodR fracR (agreeR natO).
+Definition msc_proph_total (pvs : list (val * val)) : nat :=
+  match pvs with
+  | (_, LitV (LitInt z)) :: _ => Z.to_nat z
+  | _ => 0
+  end.
+
+Lemma msc_proph_total_cons (r : nat) (pvs : list (val * val)) :
+  msc_proph_total ((#(), #(r : nat)) :: pvs) = r.
+Proof.
+  simpl. by rewrite Nat2Z.id.
+Qed.
+
+Definition msc_modelR : cmra := frac_authR (agreeR natO).
 
 Class mscG Σ := MSCG {
   msc_modelG :: inG Σ msc_modelR;
+  msc_mono_natG :: mono_natG Σ;
+  msc_request_mapG :: ghost_mapG Σ nat (nat * gname);
+  msc_saved_predG :: savedPredG Σ natO;
 }.
 
-Definition mscΣ : gFunctors := #[GFunctor msc_modelR].
+Definition mscΣ : gFunctors :=
+  #[GFunctor msc_modelR;
+    mono_natΣ;
+    ghost_mapΣ nat (nat * gname);
+    savedPredΣ natO].
 
 Global Instance subG_mscΣ Σ : subG mscΣ Σ → mscG Σ.
-Proof. solve_inG. Qed.
+Proof.
+  solve_inG.
+Qed.
 
 Definition mscN : namespace := nroot .@ "sharded_counter_modular".
+Definition mscE : coPset := ⊤.
+Lemma mscN_subset_mscE : ↑mscN ⊆ mscE.
+Proof.
+  set_solver.
+Qed.
 
-Definition msc_model_elem (q : Qp) (n : nat) : msc_modelR :=
-  (q, to_agree n).
-Typeclasses Opaque msc_model_elem.
+
+Definition msc_auth_elem (n : nat) : msc_modelR :=
+  ●F (to_agree n).
+Definition msc_frag_elem (q : Qp) (n : nat) : msc_modelR :=
+  ◯F{q} (to_agree n).
+Typeclasses Opaque msc_auth_elem msc_frag_elem.
+
 
 Section model.
   Context `{!mscG Σ}.
 
-  Global Instance msc_model_elem_fractional γ n :
-    Fractional (λ q, own γ (msc_model_elem q n))%I.
+  Global Instance msc_frag_elem_fractional γ n :
+    Fractional (λ q, own γ (msc_frag_elem q n))%I.
   Proof.
-    intros p q. rewrite /msc_model_elem -own_op.
-    f_equiv. split; first done. by rewrite /= agree_idemp.
+    intros p q. rewrite /msc_frag_elem -own_op.
+    f_equiv. by rewrite -frac_auth_frag_op agree_idemp.
   Qed.
 
-  Global Instance msc_model_elem_as_fractional γ q n :
-    AsFractional (own γ (msc_model_elem q n))
-      (λ q, own γ (msc_model_elem q n))%I q.
-  Proof. split; first done. apply _. Qed.
+  Global Instance msc_frag_elem_as_fractional γ q n :
+    AsFractional (own γ (msc_frag_elem q n))
+      (λ q, own γ (msc_frag_elem q n))%I q.
+  Proof.
+    split; first done. apply _.
+  Qed.
 End model.
 
 
 Section proof.
   Context `{!heapGS Σ, !mscG Σ}.
-  Definition msc_name : Type := gname * nat.
+  Record msc_name := MscName {
+    msc_model_name : gname;
+    msc_size : nat;
+    msc_shard_names : list gname;
+    msc_request_name : gname;
+  }.
 
-  Definition msc_model
+
+
+  Definition msc_auth (γ : msc_name) (n : nat) : iProp Σ :=
+    own γ.(msc_model_name) (msc_auth_elem n).
+  Definition msc_frag
       (γ : msc_name) (q : Qp) (n : nat) : iProp Σ :=
-    own γ.1 (msc_model_elem q n).
+    own γ.(msc_model_name) (msc_frag_elem q n).
+  Global Instance msc_frag_fractional γ n :
+    Fractional (λ q, msc_frag γ q n).
+  Proof.
+    apply _.
+  Qed.
 
-  Global Instance msc_model_fractional γ n :
-    Fractional (λ q, msc_model γ q n).
-  Proof. apply _. Qed.
+
+
+  Lemma msc_auth_frag_update γ n m k :
+    msc_auth γ n -∗ msc_frag γ 1%Qp m ==∗
+    msc_auth γ k ∗ msc_frag γ 1%Qp k.
+  Proof.
+    iIntros "Hauth Hfrag".
+    iMod (own_update_2 _ _ _
+      (msc_auth_elem k ⋅ msc_frag_elem 1%Qp k)
+      with "Hauth Hfrag") as "H".
+    { rewrite /msc_auth_elem /msc_frag_elem.
+      apply frac_auth_update_1. done. }
+    iEval (rewrite own_op) in "H".
+    iExact "H".
+  Qed.
+
+
+
+  Definition msc_shard_auth
+      (a : loc) (i n : nat) (γs : gname) : iProp Σ :=
+    (a +ₗ i) ↦ #(n : nat) ∗ mono_nat_auth_own γs 1 n.
+
+  Definition msc_shard_lb (γs : gname) (n : nat) : iProp Σ :=
+    mono_nat_lb_own γs n.
+
+
+
+
+  Definition msc_read_pending
+      (γ : msc_name) (total r : nat) (γQ : gname) : iProp Σ :=
+    ∃ (P : iProp Σ) (Q : nat → iProp Σ),
+      saved_pred_own γQ DfracDiscarded Q ∗
+      P ∗
+      □ (msc_auth γ r ∗ P
+          ={mscE ∖ ↑mscN}=∗
+         msc_auth γ r ∗ Q r) ∗
+      ⌜total < r⌝.
+
+  Definition msc_read_done
+      (total r : nat) (γQ : gname) : iProp Σ :=
+    ∃ Q : nat → iProp Σ,
+      saved_pred_own γQ DfracDiscarded Q ∗ Q r ∗ ⌜r ≤ total⌝.
+
+
+
+  Definition msc_read_state
+      (γ : msc_name) (total : nat) (request : nat * gname) : iProp Σ :=
+    msc_read_pending γ total request.1 request.2 ∨
+    msc_read_done total request.1 request.2.
+  Definition msc_requests
+      (γ : msc_name) (total : nat)
+      (requests : gmap nat (nat * gname)) : iProp Σ :=
+    ghost_map_auth γ.(msc_request_name) 1 requests ∗
+    [∗ map] _ ↦ request ∈ requests, msc_read_state γ total request.
+
+
+
+  Definition msc_shards
+      (a : loc) (ns : list nat) (γs : list gname) : iProp Σ :=
+    ([∗ list] i ↦ n ∈ ns, (a +ₗ i) ↦ #(n : nat)) ∗
+    [∗ list] _ ↦ n; γi ∈ ns; γs, mono_nat_auth_own γi 1 n.
+
+  Definition msc_lbs (ns : list nat) (γs : list gname) : iProp Σ :=
+    [∗ list] _ ↦ n; γi ∈ ns; γs, msc_shard_lb γi n.
+
+  Global Instance msc_lbs_persistent ns γs :
+    Persistent (msc_lbs ns γs).
+  Proof.
+    apply _.
+  Qed.
+
+
+  Lemma msc_read_state_advance γ n request :
+    msc_auth γ (S n) -∗
+    msc_read_state γ n request
+      ={mscE ∖ ↑mscN}=∗
+    msc_auth γ (S n) ∗ msc_read_state γ (S n) request.
+  Proof.
+    destruct request as [r γQ].
+    rewrite /msc_read_state /msc_read_pending /msc_read_done /=.
+    iIntros "Hauth [Hpending | Hdone]".
+    - iDestruct "Hpending" as (P Q) "(#HQsaved & HP & #HVS & %Hnr)".
+      destruct (decide (r = S n)) as [->|Hne].
+      + iMod ("HVS" with "[$Hauth $HP]") as "[Hauth HQ]".
+        iModIntro. iFrame "Hauth". iRight.
+        iExists Q. iFrame "HQ HQsaved". iPureIntro. lia.
+      + iModIntro. iFrame "Hauth". iLeft.
+        iExists P, Q. iFrame "HQsaved HP HVS". iPureIntro. lia.
+    - iDestruct "Hdone" as (Q) "(#HQsaved & HQ & %Hrn)".
+      iModIntro. iFrame "Hauth". iRight.
+      iExists Q. iFrame "HQ HQsaved". iPureIntro. lia.
+  Qed.
+
+  Lemma msc_read_states_advance γ n
+      (requests : gmap nat (nat * gname)) :
+    msc_auth γ (S n) -∗
+    ([∗ map] _ ↦ request ∈ requests, msc_read_state γ n request)
+      ={mscE ∖ ↑mscN}=∗
+    msc_auth γ (S n) ∗
+    [∗ map] _ ↦ request ∈ requests, msc_read_state γ (S n) request.
+  Proof.
+    induction requests as [|k request requests Hnone IH] using map_ind.
+    - rewrite !big_sepM_empty. iIntros "Hauth _".
+      iModIntro. iFrame.
+    - rewrite !big_sepM_insert //.
+      iIntros "Hauth [Hrequest Hrequests]".
+      iMod (IH with "Hauth Hrequests") as "[Hauth Hrequests]".
+      iMod (msc_read_state_advance with "Hauth Hrequest")
+        as "[Hauth Hrequest]".
+      iModIntro. iFrame.
+  Qed.
+
+  Lemma msc_requests_advance γ n requests :
+    msc_auth γ (S n) -∗ msc_requests γ n requests
+      ={mscE ∖ ↑mscN}=∗
+    msc_auth γ (S n) ∗ msc_requests γ (S n) requests.
+  Proof.
+    iIntros "Hauth [Hmap Hstates]".
+    iMod (msc_read_states_advance with "Hauth Hstates")
+      as "[$ Hstates]".
+    iModIntro. iFrame.
+  Qed.
+
+  Lemma msc_request_register γ total r γQ requests
+      (P : iProp Σ) (Q : nat → iProp Σ) :
+    total ≤ r →
+    saved_pred_own γQ DfracDiscarded Q -∗
+    □ (msc_auth γ r ∗ P
+        ={mscE ∖ ↑mscN}=∗
+       msc_auth γ r ∗ Q r) -∗
+    msc_auth γ total -∗ msc_requests γ total requests -∗ P
+      ={mscE ∖ ↑mscN}=∗
+    ∃ id : nat,
+      msc_auth γ total ∗
+      msc_requests γ total (<[id := (r, γQ)]> requests) ∗
+      id ↪[γ.(msc_request_name)] (r, γQ).
+  Proof.
+    iIntros (Htotalr) "#HQsaved #HVS Hauth [Hmap Hstates] HP".
+    set (id := fresh (dom requests)).
+    have Hid : requests !! id = None.
+    { apply not_elem_of_dom. apply is_fresh. }
+    destruct (decide (total = r)) as [->|Hne].
+    - iMod ("HVS" with "[$Hauth $HP]") as "[Hauth HQ]".
+      iAssert (msc_read_state γ r (r, γQ))
+        with "[HQ]" as "Hstate".
+      { rewrite /msc_read_state /msc_read_done /=. iRight.
+        iExists Q. iFrame "HQ HQsaved". iPureIntro. lia. }
+      iMod (ghost_map_insert id (r, γQ) with "Hmap")
+        as "[Hmap Hid]"; first done.
+      iModIntro. iExists id. iFrame "Hauth Hid".
+      rewrite /msc_requests big_sepM_insert //; iFrame.
+    - iAssert (msc_read_state γ total (r, γQ))
+        with "[HP]" as "Hstate".
+      { rewrite /msc_read_state /msc_read_pending /=. iLeft.
+        iExists P, Q. iFrame "HP HQsaved HVS". iPureIntro. lia. }
+      iMod (ghost_map_insert id (r, γQ) with "Hmap")
+        as "[Hmap Hid]"; first done.
+      iModIntro. iExists id. iFrame "Hauth Hid".
+      rewrite /msc_requests big_sepM_insert //; iFrame.
+  Qed.
+
+  Lemma msc_request_take γ total r γQ id requests
+      (Q : nat → iProp Σ) :
+    r ≤ total →
+    saved_pred_own γQ DfracDiscarded Q -∗
+    id ↪[γ.(msc_request_name)] (r, γQ) -∗
+    msc_requests γ total requests ==∗
+    msc_requests γ total (delete id requests) ∗ ▷ Q r.
+  Proof.
+    iIntros (Hrtotal) "#HQsaved Hid [Hmap Hstates]".
+    iDestruct (ghost_map_lookup with "Hmap Hid") as %Hlookup.
+    iEval (rewrite (big_sepM_delete _ requests id (r, γQ) Hlookup))
+      in "Hstates".
+    iDestruct "Hstates" as "[Hstate Hstates]".
+    iEval (rewrite /msc_read_state /msc_read_pending /msc_read_done /=)
+      in "Hstate".
+    iDestruct "Hstate" as "[Hpending | Hdone]".
+    - iDestruct "Hpending" as (P Q') "(_ & _ & _ & %Hlt)".
+      exfalso. lia.
+    - iDestruct "Hdone" as (Q') "(#HQsaved' & HQ' & _)".
+      iPoseProof (saved_pred_agree _ _ _ _ _ r
+        with "HQsaved HQsaved'") as "Heq".
+      iAssert (▷ Q r)%I with "[HQ' Heq]" as "HQ".
+      { iNext. iRewrite "Heq". iExact "HQ'". }
+      iMod (ghost_map_delete with "Hmap Hid") as "Hmap".
+      iModIntro. iFrame "HQ".
+      rewrite /msc_requests. iFrame.
+  Qed.
+
+  Lemma msc_mono_alloc_zeros T :
+    ⊢ |==> ∃ γs : list gname,
+      ⌜length γs = T⌝ ∗
+      [∗ list] γi ∈ γs, mono_nat_auth_own γi 1 0.
+  Proof.
+    (* Induct on the requested number of ghost names. *)
+    induction T as [|T IH].
+    (* Zero shards require no allocations. *)
+    - iModIntro. iExists []. simpl. auto.
+    (* Prepend one fresh zero authority to the recursively allocated list. *)
+    - iMod IH as (γs) "[%Hlen Hγs]".
+      iMod (mono_nat_own_alloc 0) as (γi) "[Hγi _]".
+      iModIntro. iExists (γi :: γs). simpl.
+      iFrame. iPureIntro. lia.
+  Qed.
+
+
+
+
 
 
   Definition msc_inv (γ : msc_name) (a : loc) : iProp Σ :=
-    ∃ ns : list nat,
-      ⌜length ns = γ.2⌝ ∗
-      msc_model γ (1 / 2)%Qp (sum_list ns) ∗
-      [∗ list] i ↦ n ∈ ns, (a +ₗ i) ↦ #(n : nat).
+    ∃ (ns : list nat) (requests : gmap nat (nat * gname)),
+      ⌜length ns = γ.(msc_size)⌝ ∗
+      ⌜length γ.(msc_shard_names) = γ.(msc_size)⌝ ∗
+      msc_auth γ (sum_list ns) ∗
+      msc_shards a ns γ.(msc_shard_names) ∗
+      msc_requests γ (sum_list ns) requests.
 
   Definition msc_is_counter
       (γ : msc_name) (c : val) : iProp Σ :=
     ∃ a : loc,
-      ⌜c = (#a, #(γ.2 : nat))%V⌝ ∗
+      ⌜c = (#a, #(γ.(msc_size) : nat))%V⌝ ∗
       inv mscN (msc_inv γ a).
 
   Global Instance msc_is_counter_persistent γ c :
     Persistent (msc_is_counter γ c).
-  Proof. apply _. Qed.
+  Proof.
+    apply _.
+  Qed.
 
   Definition msc_handle (γ : msc_name) (h : val) : iProp Σ :=
-    ∃ i : nat, ⌜h = #(i : nat)⌝ ∗ ⌜i < γ.2⌝.
+    ∃ i : nat, ⌜h = #(i : nat)⌝ ∗ ⌜i < γ.(msc_size)⌝.
 
   Global Instance msc_handle_persistent γ h :
     Persistent (msc_handle γ h).
-  Proof. apply _. Qed.
+  Proof.
+    apply _.
+  Qed.
 
 
 
-  Lemma msc_make_handles γt T :
-    ⊢ [∗ list] i ∈ seq 0 T, msc_handle (γt, T) #(i : nat).
+
+  Lemma msc_make_handles γ :
+    ⊢ [∗ list] i ∈ seq 0 γ.(msc_size), msc_handle γ #(i : nat).
   Proof.
     iApply big_sepL_intro.
     iIntros "!>" (k i Hlookup).
@@ -122,24 +384,179 @@ Section proof.
 
 
 
-  Lemma msc_new_counter_spec E (T : nat) :
-    ↑mscN ⊆ E →
+
+  Lemma msc_load_shard γ a (i : nat) γi n0 :
+    γ.(msc_shard_names) !! i = Some γi →
+    {{{ inv mscN (msc_inv γ a) ∗ msc_shard_lb γi n0 }}}
+      ! #(a +ₗ i) @ mscE
+    {{{ (n : nat), RET #(n : nat);
+        msc_shard_lb γi n ∗ ⌜n0 ≤ n⌝ }}}.
+  Proof.
+    iIntros (Hγi Φ) "[#Hinv #Hn0] HΦ".
+    iInv mscN as (ns requests)
+      "(>%Hlen & >%Hγlen & >Hauth & >Hshards & Hrequests)" "Hclose".
+    iDestruct "Hshards" as "[Hcells Hmonos]".
+    have Hi_ns : i < length ns.
+    { have Hi_γs := lookup_lt_Some _ _ _ Hγi. lia. }
+    destruct (lookup_lt_is_Some_2 ns i Hi_ns) as [n Hn].
+    iDestruct (big_sepL_insert_acc _ _ _ _ Hn with "Hcells")
+      as "[Hl Hcells]".
+    iDestruct (big_sepL2_lookup_acc _ _ _ i n γi Hn Hγi with "Hmonos")
+      as "[Hmono Hmonos]".
+    iDestruct (mono_nat_lb_own_valid with "Hmono Hn0") as %[_ Hn0n].
+    iPoseProof (mono_nat_lb_own_get with "Hmono") as "#Hn".
+    wp_load.
+    iDestruct ("Hcells" $! n with "Hl") as "Hcells".
+    iEval (rewrite (list_insert_id _ _ _ Hn)) in "Hcells".
+    iDestruct ("Hmonos" with "Hmono") as "Hmonos".
+    iMod ("Hclose" with "[Hauth Hcells Hmonos Hrequests]") as "_".
+    { iNext. iExists ns, requests.
+      iSplit; first done.
+      iSplit; first done.
+      iSplitL "Hauth"; first done.
+      iSplitL "Hcells Hmonos".
+      { rewrite /msc_shards. iSplitL "Hcells".
+        - iExact "Hcells".
+        - iExact "Hmonos". }
+      iExact "Hrequests". }
+    iModIntro. iApply ("HΦ" $! n). iFrame "Hn". done.
+  Qed.
+
+  Lemma msc_monos_snapshot ns γs :
+    ([∗ list] _ ↦ n; γi ∈ ns; γs, mono_nat_auth_own γi 1 n) -∗
+    ([∗ list] _ ↦ n; γi ∈ ns; γs, mono_nat_auth_own γi 1 n) ∗
+    msc_lbs ns γs.
+  Proof.
+    iIntros "Hmonos".
+    iPoseProof (big_sepL2_mono with "Hmonos") as "#Hlbs".
+    { iIntros (i n γi Hn Hγi) "Hmono".
+      iApply mono_nat_lb_own_get. iExact "Hmono". }
+    iFrame "Hmonos Hlbs".
+  Qed.
+
+  Lemma msc_sum_loop_bounds γ a
+      (T i acc : nat) (lower : list nat) :
+    length lower = T →
+    length γ.(msc_shard_names) = T →
+    i ≤ T →
+    {{{ inv mscN (msc_inv γ a) ∗
+        msc_lbs lower γ.(msc_shard_names) }}}
+      msc_sum_loop #a #T #(i : nat) #(acc : nat) @ mscE
+    {{{ (r : nat), RET #(r : nat);
+        ∃ read_values : list nat,
+          ⌜length read_values = T - i⌝ ∗
+          ⌜r = (acc + sum_list read_values)%nat⌝ ∗
+          ⌜(sum_list (drop i lower) ≤ sum_list read_values)%nat⌝ ∗
+          msc_lbs read_values (drop i γ.(msc_shard_names)) }}}.
+  Proof.
+    intros Hlower Hγlen Hi.
+    remember (T - i) as fuel eqn:Hfuel.
+    revert i acc Hi Hfuel.
+    induction fuel as [|fuel IH]; intros i acc Hi Hfuel.
+    - have -> : i = T by lia.
+      iIntros (Φ) "[#Hinv #Hlowerlbs] HΦ".
+      rewrite /msc_sum_loop. wp_rec. wp_pures.
+      rewrite bool_decide_eq_true_2; last done. wp_if.
+      iApply ("HΦ" $! acc).
+      have Hdrop_lower : drop T lower = [] by apply drop_ge; lia.
+      have Hdrop_names : drop T γ.(msc_shard_names) = [] by
+        apply drop_ge; lia.
+      iExists []. rewrite Hdrop_lower Hdrop_names /msc_lbs /=.
+      auto.
+    - have Hit : i < T by lia.
+      have HiS : S i ≤ T by lia.
+      have HfuelS : fuel = T - S i by lia.
+      have Hi1 : i + 1 ≤ T by lia.
+      have Hfuel1 : fuel = T - (i + 1) by lia.
+      destruct (lookup_lt_is_Some_2 lower i) as [n0 Hn0];
+        first by rewrite Hlower.
+      destruct (lookup_lt_is_Some_2 γ.(msc_shard_names) i) as [γi Hγi];
+        first by rewrite Hγlen.
+      iIntros (Φ) "[#Hinv #Hlowerlbs] HΦ".
+      iPoseProof (big_sepL2_lookup _ _ _ i n0 γi Hn0 Hγi
+        with "Hlowerlbs") as "#Hn0".
+      rewrite /msc_sum_loop. wp_rec. wp_pures.
+      rewrite bool_decide_eq_false_2; last naive_solver lia. wp_if.
+      wp_pures.
+      wp_bind (! _)%E.
+      wp_apply (msc_load_shard γ a i γi n0 with "[$Hinv $Hn0]");
+        first done.
+      iIntros (n) "[#Hn %Hn0n]".
+      wp_let.
+      fold msc_sum_loop.
+      wp_bind (msc_sum_loop #a #T
+        (#(i : nat) + #1) (#(acc : nat) + #(n : nat)))%E.
+      wp_binop. rewrite -Nat2Z.inj_add.
+      wp_binop.
+      replace (Z.of_nat i + 1)%Z with (Z.of_nat (i + 1)) by lia.
+      wp_apply (IH (i + 1) (acc + n) Hi1 Hfuel1
+        with "[$Hinv $Hlowerlbs]").
+      iIntros (r) "Hpost".
+      iDestruct "Hpost" as (read_values)
+        "(%Hreadlen & %Hr & %Hlowerread & #Hreadlbs)".
+      rewrite Nat.add_1_r in Hreadlen, Hlowerread.
+      iEval (rewrite Nat.add_1_r) in "Hreadlbs".
+      iApply ("HΦ" $! r).
+      iExists (n :: read_values).
+      iSplit.
+      { iPureIntro. simpl. rewrite Hreadlen. lia. }
+      iSplit.
+      { iPureIntro. simpl. lia. }
+      rewrite (drop_S lower n0 i Hn0).
+      iSplit.
+      { iPureIntro. simpl. lia. }
+      rewrite (drop_S γ.(msc_shard_names) γi i Hγi).
+      rewrite /msc_lbs /=. iFrame "Hn Hreadlbs".
+  Qed.
+
+  Lemma msc_lbs_sum_le xs ys γs :
+    length xs = length γs →
+    length ys = length γs →
+    msc_lbs xs γs -∗
+    ([∗ list] _ ↦ n; γi ∈ ys; γs, mono_nat_auth_own γi 1 n) -∗
+    ⌜sum_list xs ≤ sum_list ys⌝.
+  Proof.
+    revert ys γs.
+    induction xs as [|x xs IH]; intros [|y ys] [|γi γs] Hxs Hys;
+      simpl in Hxs, Hys; try lia.
+    - rewrite /msc_lbs /=. iIntros "_ _". done.
+    - rewrite /msc_lbs /=.
+      iIntros "[#Hx Hxs] [Hy Hys]".
+      iDestruct (mono_nat_lb_own_valid with "Hy Hx") as %[_ Hxy].
+      have Hxs' : length xs = length γs by lia.
+      have Hys' : length ys = length γs by lia.
+      iDestruct (IH ys γs Hxs' Hys' with "Hxs Hys") as %Hsum.
+      iPureIntro. simpl. lia.
+  Qed.
+
+
+
+
+
+
+  Lemma msc_new_counter_spec (T : nat) :
     {{{ ⌜0 < T⌝ }}}
-      msc_new_counter #T @ E
+      msc_new_counter #T @ mscE
     {{{ c γ, RET c;
         msc_is_counter γ c ∗
         ([∗ list] i ∈ seq 0 T,
           msc_handle γ #(i : nat)) ∗
-        msc_model γ (1 / 2)%Qp 0 }}}.
+        msc_frag γ 1%Qp 0 }}}.
   Proof.
-    iIntros (Hsubset Φ) "%HT HΦ".
+    iIntros (Φ) "%HT HΦ".
     rewrite /msc_new_counter. wp_lam.
     wp_alloc a as "Ha"; first lia.
     iEval (rewrite Nat2Z.id) in "Ha".
 
-    iMod (own_alloc (msc_model_elem 1%Qp 0)) as (γt) "Hmodel";
-      first done.
-    iDestruct "Hmodel" as "[Hinternal Hclient]".
+    iMod (own_alloc (msc_auth_elem 0 ⋅ msc_frag_elem 1%Qp 0))
+      as (γt) "[Hauth Hfrag]".
+    { rewrite /msc_auth_elem /msc_frag_elem.
+      apply frac_auth_valid. done. }
+
+    iMod (ghost_map_alloc_empty (K:=nat) (V:=nat * gname))
+      as (γreq) "Hrequests".
+    iMod (msc_mono_alloc_zeros T) as (γs) "[%Hγslen Hγs]".
+    set (γ := MscName γt T γs γreq).
 
     iAssert ([∗ list] i ↦ n ∈ replicate T (0 : nat),
         (a +ₗ i) ↦ #(n : nat))%I with "[Ha]" as "Hcells".
@@ -147,35 +564,41 @@ Section proof.
           (λ i v, (a +ₗ i) ↦ v)%I (replicate T (0 : nat))).
       rewrite fmap_replicate /array. iFrame. }
 
-    iMod (inv_alloc mscN _ (msc_inv (γt, T) a)
-      with "[Hinternal Hcells]") as "#Hinv".
-    { iNext. iExists (replicate T (0 : nat)).
-      iSplit; first by rewrite length_replicate.
-      rewrite sum_list_replicate Nat.mul_0_r. iFrame. }
+    iAssert (msc_shards a (replicate T (0 : nat)) γs)
+      with "[Hcells Hγs]" as "Hshards".
+    { rewrite /msc_shards.
+      iFrame "Hcells".
+      rewrite big_sepL2_replicate_l; first iExact "Hγs".
+      done. }
 
-    iPoseProof (msc_make_handles γt T) as "Hhandles".
+    iMod (inv_alloc mscN _ (msc_inv γ a)
+      with "[Hauth Hshards Hrequests]") as "#Hinv".
+    { iNext. iExists (replicate T (0 : nat)), (∅ : gmap nat (nat * gname)).
+      iSplit; first by rewrite length_replicate.
+      iSplit; first done.
+      rewrite sum_list_replicate Nat.mul_0_r.
+      rewrite /msc_requests big_sepM_empty. iFrame. }
+
+    iPoseProof (msc_make_handles γ) as "Hhandles".
     wp_pures.
-    iApply ("HΦ" $! (#a, #T)%V (γt, T)).
-    iFrame "Hhandles Hclient".
+    iApply ("HΦ" $! (#a, #T)%V γ).
+    iFrame "Hhandles Hfrag".
     iExists a. iFrame "Hinv". done.
   Qed.
 
-
-
   Lemma msc_incr_spec
-      E γ c h (P : iProp Σ) (Q : nat → iProp Σ) :
-    ↑mscN ⊆ E →
+      γ c h (P : iProp Σ) (Q : nat → iProp Σ) :
     (∀ total,
-      □ (msc_model γ (1 / 2)%Qp total ∗ P
-          ={E ∖ ↑mscN}=∗
-         msc_model γ (1 / 2)%Qp (S total) ∗ Q total)) ⊢
+      □ (msc_auth γ total ∗ P
+          ={mscE ∖ ↑mscN}=∗
+         msc_auth γ (S total) ∗ Q total)) ⊢
     {{{ msc_is_counter γ c ∗ msc_handle γ h ∗ P }}}
-      msc_incr c h @ E
+      msc_incr c h @ mscE
     {{{ RET #();
         msc_is_counter γ c ∗ msc_handle γ h ∗
         ∃ total, Q total }}}.
   Proof.
-    iIntros (Hsubset) "#HVS".
+    iIntros "#HVS".
     iIntros (Φ) "!# (#Hcounter & #Hhandle & HP) HΦ".
     iDestruct "Hcounter" as (a ->) "#Hinv".
     iDestruct "Hhandle" as (i) "[%Hh %Hi]".
@@ -183,23 +606,38 @@ Section proof.
 
     rewrite /msc_incr. wp_lam. wp_pures.
     wp_bind (FAA _ _)%E.
-    iInv mscN as (ns) ">(%Hlen & Hmodel & Hcells)" "Hclose".
+    iInv mscN as (ns requests)
+      "(>%Hlen & >%Hγlen & >Hauth & >Hshards & Hrequests)" "Hclose".
+    iDestruct "Hshards" as "[Hcells Hmonos]".
 
     have Hi_ns : i < length ns by lia.
     destruct (lookup_lt_is_Some_2 ns i Hi_ns) as [n Hn].
+    have Hi_γs : i < length γ.(msc_shard_names) by lia.
+    destruct (lookup_lt_is_Some_2 γ.(msc_shard_names) i Hi_γs)
+      as [γi Hγi].
     iDestruct (big_sepL_insert_acc _ _ _ _ Hn with "Hcells")
       as "[Hl Hcells]".
+    iDestruct (big_sepL2_insert_acc _ _ _ i n γi Hn Hγi with "Hmonos")
+      as "[Hmono Hmonos]".
 
     wp_faa.
-    iMod ("HVS" $! (sum_list ns) with "[$Hmodel $HP]")
-      as "[Hmodel HQ]".
+    iMod (mono_nat_own_update (S n) with "Hmono")
+      as "[Hmono _]"; first lia.
+    iMod ("HVS" $! (sum_list ns) with "[$Hauth $HP]")
+      as "[Hauth HQ]".
+    iMod (msc_requests_advance γ (sum_list ns) requests
+      with "Hauth Hrequests") as "[Hauth Hrequests]".
 
     iEval (rewrite Z.add_1_r -Nat2Z.inj_succ) in "Hl".
     iDestruct ("Hcells" $! (S n) with "Hl") as "Hcells".
-    iMod ("Hclose" with "[Hmodel Hcells]") as "_".
-    { iNext. iExists (<[i := S n]> ns).
+    iDestruct ("Hmonos" $! (S n) γi with "Hmono") as "Hmonos".
+    iEval (rewrite (list_insert_id _ _ _ Hγi)) in "Hmonos".
+    iMod ("Hclose" with "[Hauth Hcells Hmonos Hrequests]") as "_".
+    { iNext. iExists (<[i := S n]> ns), requests.
       iSplit; first by rewrite length_insert.
-      rewrite (msc_sum_list_insert_S _ _ _ Hn). iFrame. }
+      iSplit; first done.
+      rewrite (msc_sum_list_insert_S _ _ _ Hn).
+      rewrite /msc_shards. iFrame. }
 
     iModIntro. wp_pures.
     iApply "HΦ".
@@ -211,21 +649,120 @@ Section proof.
     iExists (sum_list ns). iFrame.
   Qed.
 
-
   Lemma msc_read_spec
-      E γ c (P : iProp Σ) (Q : nat → iProp Σ) :
-    ↑mscN ⊆ E →
+      γ c (P : iProp Σ) (Q : nat → iProp Σ) :
     (∀ total,
-      □ (msc_model γ (1 / 2)%Qp total ∗ P
-          ={E ∖ ↑mscN}=∗
-         msc_model γ (1 / 2)%Qp total ∗ Q total)) ⊢
+      □ (msc_auth γ total ∗ P
+          ={mscE ∖ ↑mscN}=∗
+         msc_auth γ total ∗ Q total)) ⊢
     {{{ msc_is_counter γ c ∗ P }}}
-      msc_read c @ E
+      msc_read c @ mscE
     {{{ (total : nat), RET #total;
         msc_is_counter γ c ∗ Q total }}}.
   Proof.
-  Admitted.
+    iIntros "#HVS".
+    iIntros (Φ) "!# (#Hcounter & HP) HΦ".
+    iDestruct "Hcounter" as (a ->) "#Hinv".
+    iMod (saved_pred_alloc Q DfracDiscarded) as (γQ) "#HQsaved";
+      first done.
 
+    rewrite /msc_read. wp_lam.
+    wp_bind NewProph.
+    iInv mscN as (initial requests)
+      "(>%Hlen & >%Hγlen & >Hauth & >Hshards & Hrequests)" "Hclose".
+    iDestruct "Hshards" as "[Hcells Hmonos]".
+    iDestruct (msc_monos_snapshot with "Hmonos")
+      as "[Hmonos #Hinitiallbs]".
+    wp_apply wp_new_proph; first done.
+    iIntros (pvs p) "Hp".
+    set (predicted := msc_proph_total pvs).
+    iPoseProof ("HVS" $! predicted) as "#HVSpredicted".
+
+    iAssert (|={mscE ∖ ↑mscN}=> ∃ current_requests : gmap nat (nat * gname),
+        msc_auth γ (sum_list initial) ∗
+        msc_requests γ (sum_list initial) current_requests ∗
+        ((⌜sum_list initial ≤ predicted⌝ ∗
+          ∃ id : nat,
+            id ↪[γ.(msc_request_name)] (predicted, γQ)) ∨
+         (⌜predicted < sum_list initial⌝ ∗ P)))%I
+      with "[HP Hauth Hrequests]" as "Hregistered".
+    { destruct (decide (sum_list initial ≤ predicted)) as [Hle|Hlt].
+      - iMod (msc_request_register γ (sum_list initial) predicted γQ
+          requests P Q Hle with "HQsaved HVSpredicted Hauth Hrequests HP")
+          as (id) "(Hauth & Hrequests & Hid)".
+        iModIntro. iExists (<[id := (predicted, γQ)]> requests).
+        iFrame "Hauth Hrequests". iLeft.
+        iSplit; first done. iExists id. iExact "Hid".
+      - iModIntro. iExists requests. iFrame "Hauth Hrequests".
+        iRight. iFrame. iPureIntro. lia. }
+    iMod "Hregistered" as (current_requests)
+      "(Hauth & Hrequests & Hcase)".
+
+    iMod ("Hclose" with "[Hauth Hcells Hmonos Hrequests]") as "_".
+    { iNext. iExists initial, current_requests.
+      iSplit; first done. iSplit; first done.
+      iSplitL "Hauth"; first done.
+      iSplitL "Hcells Hmonos".
+      { rewrite /msc_shards. iFrame. }
+      iExact "Hrequests". }
+    iModIntro.
+
+    wp_pures.
+    wp_apply (msc_sum_loop_bounds γ a γ.(msc_size) 0 0 initial
+      Hlen Hγlen with "[$Hinv $Hinitiallbs]"); first lia.
+    iIntros (actual) "Hscan".
+    iDestruct "Hscan" as (read_values)
+      "(%Hreadlen & %Hactual & %Hlower & #Hreadlbs)".
+    rewrite drop_0 in Hlower.
+    iEval (rewrite drop_0) in "Hreadlbs".
+    have Hinitial_actual : sum_list initial ≤ actual by lia.
+    wp_let.
+
+    iDestruct "Hcase" as
+      "[(%Hinitial_predicted & Hid) | (%Hpredicted_initial & HP)]".
+    - iDestruct "Hid" as (id) "Hid".
+      wp_bind (ResolveProph #p #(actual : nat))%E.
+      iInv "Hinv" as (final requests') "(>%Hfinallen & >%Hγlen' &
+        >Hauth & >Hshards & Hrequests)" "Hclose".
+      iDestruct "Hshards" as "[Hcells Hmonos]".
+      have Hreadnames :
+        length read_values = length γ.(msc_shard_names) by lia.
+      have Hfinalnames :
+        length final = length γ.(msc_shard_names) by lia.
+      iDestruct (msc_lbs_sum_le read_values final γ.(msc_shard_names)
+        Hreadnames Hfinalnames with "Hreadlbs Hmonos")
+        as %Hactual_final.
+      wp_apply (wp_resolve_proph with "[Hp]")
+        as (pvs') "[%Hpvs Hp]"; first done.
+      have Hpredicted_actual : predicted = actual.
+      { subst pvs. apply msc_proph_total_cons. }
+      subst predicted.
+      iEval (rewrite Hpredicted_actual) in "Hid".
+      have Hactual_final' : actual ≤ sum_list final by lia.
+      iMod (msc_request_take γ (sum_list final) actual γQ id requests' Q
+        Hactual_final' with "HQsaved Hid Hrequests")
+        as "[Hrequests HQ]".
+
+      iMod ("Hclose" with "[Hauth Hcells Hmonos Hrequests]") as "_".
+      { iNext. iExists final, (delete id requests').
+        iSplit; first done. iSplit; first done.
+        iSplitL "Hauth"; first done.
+        iSplitL "Hcells Hmonos".
+        { rewrite /msc_shards. iFrame. }
+        iExact "Hrequests". }
+      iModIntro. wp_seq.
+      iApply ("HΦ" $! actual).
+      iModIntro.
+      iSplit; first (iExists a; iFrame "Hinv"; done).
+      iExact "HQ".
+
+    - wp_bind (ResolveProph #p #(actual : nat))%E.
+      wp_apply (wp_resolve_proph with "[Hp]")
+        as (pvs') "[%Hpvs Hp]"; first done.
+      have Hpredicted_actual : predicted = actual.
+      { subst pvs. apply msc_proph_total_cons. }
+      exfalso. lia.
+  Qed.
 
   Definition modular_sharded_counter : modular_counter Σ := {|
     modular_new_counter := msc_new_counter;
@@ -233,15 +770,201 @@ Section proof.
     modular_read := msc_read;
     modular_counter_name := msc_name;
     modular_counter_namespace := mscN;
+    modular_counter_mask := mscE;
+    modular_counter_namespace_subset := mscN_subset_mscE;
     modular_is_counter := msc_is_counter;
     modular_handle := msc_handle;
-    counter_model := msc_model;
+    counter_auth := msc_auth;
+    counter_frag := msc_frag;
     modular_is_counter_persistent := msc_is_counter_persistent;
     modular_handle_persistent := msc_handle_persistent;
-    counter_model_fractional := msc_model_fractional;
+    counter_frag_fractional := msc_frag_fractional;
     modular_new_counter_spec := msc_new_counter_spec;
     modular_incr_spec := msc_incr_spec;
     modular_read_spec := msc_read_spec;
   |}.
+
+
+
+
+
+  Definition msc_incr_twice : val :=
+    λ: "c" "h", msc_incr "c" "h";; msc_incr "c" "h".
+  Definition msc_two_incr_twice_read : val :=
+    λ: "c" "h1" "h2",
+      (msc_incr_twice "c" "h1" ||| msc_incr_twice "c" "h2");;
+      msc_read "c".
+
+  Definition msc_clientN : namespace :=
+    nroot .@ "sharded_counter_modular_client".
+
+  Definition msc_client_inv
+      (γ : msc_name) (γm γd : gname) (n : nat) : iProp Σ :=
+    (∃ k1 k2 : nat,
+       ghost_map_auth γm 1
+         (<[1 := (k1, γd)]> (<[2 := (k2, γd)]>
+            (∅ : gmap nat (nat * gname)))) ∗
+       msc_frag γ 1%Qp (n + k1 + k2)) ∨
+    ghost_map_auth γm 1 (∅ : gmap nat (nat * gname)).
+
+  Lemma msc_auth_frag_agree γ (t m : nat) :
+    msc_auth γ t -∗ msc_frag γ 1%Qp m -∗ ⌜t = m⌝.
+  Proof.
+    iIntros "Hauth Hfrag".
+    iDestruct (own_valid_2 with "Hauth Hfrag") as %Hvalid.
+    iPureIntro.
+    rewrite /msc_auth_elem /msc_frag_elem in Hvalid.
+    apply frac_auth_agree in Hvalid.
+    apply (inj to_agree), leibniz_equiv in Hvalid.
+    exact Hvalid.
+  Qed.
+
+  Lemma msc_client_incr_spec γ c h (γm γd : gname) (n i ki : nat) :
+    i = 1 ∨ i = 2 →
+    {{{ inv msc_clientN (msc_client_inv γ γm γd n) ∗
+        msc_is_counter γ c ∗
+        msc_handle γ h ∗
+        i ↪[γm] (ki, γd) }}}
+      msc_incr c h
+    {{{ RET #(); i ↪[γm] (S ki, γd) }}}.
+  Proof.
+    iIntros (Hi Φ) "(#HclientInv & #Hcounter & #Hhandle & Helem) HΦ".
+    iPoseProof (msc_incr_spec γ c h
+        (i ↪[γm] (ki, γd))%I
+        (λ _ : nat, i ↪[γm] (S ki, γd))%I
+      with "[]") as "#Hincr".
+    { iIntros (total) "!> [Hauth Helem]".
+      rewrite /mscE.
+      iInv msc_clientN as
+        "[(%k1 & %k2 & >Hmap & >Hfrag) | >Hempty]" "Hclose"; last first.
+      { iDestruct (ghost_map_lookup with "Hempty Helem") as %Hbad.
+        rewrite lookup_empty in Hbad. discriminate Hbad. }
+      iDestruct (ghost_map_lookup with "Hmap Helem") as %Hlookup.
+      iDestruct (msc_auth_frag_agree with "Hauth Hfrag") as %->.
+      iMod (msc_auth_frag_update γ _ _ (S (n + k1 + k2))
+        with "Hauth Hfrag") as "[Hauth Hfrag]".
+      iMod (ghost_map_update (S ki, γd) with "Hmap Helem")
+        as "[Hmap Helem]".
+      destruct Hi as [-> | ->].
+      - rewrite lookup_insert_eq in Hlookup.
+        assert (k1 = ki) as -> by congruence.
+        iEval (rewrite insert_insert_eq) in "Hmap".
+        iMod ("Hclose" with "[Hmap Hfrag]") as "_".
+        { iNext. iLeft. iExists (S ki), k2.
+          have -> : n + S ki + k2 = S (n + ki + k2) by lia.
+          iFrame. }
+        iModIntro. iFrame.
+      - rewrite lookup_insert_ne in Hlookup; last lia.
+        rewrite lookup_insert_eq in Hlookup.
+        assert (k2 = ki) as -> by congruence.
+        have Hmapeq :
+          <[2 := (S ki, γd)]> (<[1 := (k1, γd)]> (<[2 := (ki, γd)]>
+            (∅ : gmap nat (nat * gname))))
+          = <[1 := (k1, γd)]> (<[2 := (S ki, γd)]> ∅).
+        { rewrite insert_insert_ne; last lia.
+          by rewrite insert_insert_eq. }
+        iEval (rewrite Hmapeq) in "Hmap".
+        iMod ("Hclose" with "[Hmap Hfrag]") as "_".
+        { iNext. iLeft. iExists k1, (S ki).
+          have -> : n + k1 + S ki = S (n + k1 + ki) by lia.
+          iFrame. }
+        iModIntro. iFrame. }
+    wp_apply ("Hincr" with "[$Hcounter $Hhandle $Helem]").
+    iIntros "(_ & _ & (%total & Helem))".
+    iApply "HΦ". iFrame.
+  Qed.
+
+  Lemma msc_two_incr_twice_read_spec `{!spawnG Σ} γ c h1 h2 n :
+    {{{ msc_is_counter γ c ∗
+        msc_handle γ h1 ∗
+        msc_handle γ h2 ∗
+        msc_frag γ 1%Qp n }}}
+      msc_two_incr_twice_read c h1 h2
+    {{{ RET #(n + 4 : nat);
+        msc_is_counter γ c ∗
+        msc_handle γ h1 ∗
+        msc_handle γ h2 ∗
+        msc_frag γ 1%Qp (n + 4) }}}.
+  Proof.
+    iIntros (Φ) "(#Hcounter & #Hh1 & #Hh2 & Hfrag) HΦ".
+    set (γd := γ.(msc_model_name)).
+
+    iMod (ghost_map_alloc_empty (K:=nat) (V:=nat * gname)) as (γm) "Hmap".
+    iMod (ghost_map_insert 2 (0, γd) with "Hmap") as "[Hmap Helem2]";
+      first apply lookup_empty.
+    iMod (ghost_map_insert 1 (0, γd) with "Hmap") as "[Hmap Helem1]";
+      first (rewrite lookup_insert_ne; [apply lookup_empty | lia]).
+    iMod (inv_alloc msc_clientN _ (msc_client_inv γ γm γd n)
+      with "[Hmap Hfrag]") as "#HclientInv".
+    { iNext. iLeft. iExists 0, 0.
+      rewrite !Nat.add_0_r. iFrame. }
+
+    rewrite /msc_two_incr_twice_read.
+    wp_smart_apply (wp_par
+        (λ _, 1 ↪[γm] ((2 : nat), γd))%I
+        (λ _, 2 ↪[γm] ((2 : nat), γd))%I
+      with "[Helem1] [Helem2]").
+    - rewrite /msc_incr_twice.
+      wp_smart_apply (msc_client_incr_spec γ c h1 γm γd n 1 0
+          (or_introl eq_refl)
+        with "[$HclientInv $Hcounter $Hh1 $Helem1]") as "Helem1".
+      wp_smart_apply (msc_client_incr_spec γ c h1 γm γd n 1 1
+          (or_introl eq_refl)
+        with "[$HclientInv $Hcounter $Hh1 $Helem1]") as "Helem1".
+      done.
+    - rewrite /msc_incr_twice.
+      wp_smart_apply (msc_client_incr_spec γ c h2 γm γd n 2 0
+          (or_intror eq_refl)
+        with "[$HclientInv $Hcounter $Hh2 $Helem2]") as "Helem2".
+      wp_smart_apply (msc_client_incr_spec γ c h2 γm γd n 2 1
+          (or_intror eq_refl)
+        with "[$HclientInv $Hcounter $Hh2 $Helem2]") as "Helem2".
+      done.
+    - iIntros (v1 v2) "[Helem1 Helem2] !>".
+      iPoseProof (msc_read_spec γ c
+          (1 ↪[γm] ((2 : nat), γd) ∗ 2 ↪[γm] ((2 : nat), γd))%I
+          (λ total : nat,
+            ⌜total = (n + 4)%nat⌝ ∗ msc_frag γ 1%Qp (n + 4))%I
+        with "[]") as "#Hread".
+      { iIntros (total) "!> [Hauth [Helem1 Helem2]]".
+        rewrite /mscE.
+        iInv msc_clientN as
+          "[(%k1 & %k2 & >Hmap & >Hfrag) | >Hempty]" "Hclose"; last first.
+        { iDestruct (ghost_map_lookup with "Hempty Helem1") as %Hbad.
+          rewrite lookup_empty in Hbad. discriminate Hbad. }
+        iDestruct (ghost_map_lookup with "Hmap Helem1") as %Hl1.
+        iDestruct (ghost_map_lookup with "Hmap Helem2") as %Hl2.
+        rewrite lookup_insert_eq in Hl1.
+        rewrite lookup_insert_ne in Hl2; last lia.
+        rewrite lookup_insert_eq in Hl2.
+        assert (k1 = 2) as -> by congruence.
+        assert (k2 = 2) as -> by congruence.
+        iDestruct (msc_auth_frag_agree with "Hauth Hfrag") as %Htotal.
+        iMod (ghost_map_delete with "Hmap Helem1") as "Hmap".
+        iMod (ghost_map_delete with "Hmap Helem2") as "Hmap".
+        have Hdel :
+          delete 2 (delete 1 (<[1 := ((2 : nat), γd)]>
+            (<[2 := ((2 : nat), γd)]> (∅ : gmap nat (nat * gname)))))
+          = ∅.
+        { rewrite delete_insert_eq.
+          rewrite delete_insert_ne; last lia.
+          rewrite delete_empty delete_insert_eq.
+          by rewrite delete_empty. }
+        iEval (rewrite Hdel) in "Hmap".
+        iMod ("Hclose" with "[Hmap]") as "_".
+        { iNext. iRight. iFrame. }
+        iModIntro.
+        have Heq : n + 2 + 2 = n + 4 by lia.
+        iEval (rewrite Heq) in "Hfrag".
+        iFrame "Hauth Hfrag".
+        iPureIntro. lia. }
+      wp_smart_apply ("Hread" with "[$Hcounter $Helem1 $Helem2]").
+      iIntros (total) "(_ & %Htotal & Hfrag)".
+      subst total.
+      iApply "HΦ".
+      by iFrame "Hcounter Hh1 Hh2 Hfrag".
+  Qed.
+
+
 
 End proof.
