theories/counter_spec_modular.v
@@ -6,15 +6,27 @@ From iris.prelude Require Import options.
 
 Class modular_counter (Σ : gFunctors) `{!heapGS Σ} := ModularCounter {
   modular_new_counter : val;
+
   modular_incr : val;
+
   modular_read : val;
 
   modular_counter_name : Type;
+
   modular_counter_namespace : namespace;
 
+  modular_counter_mask : coPset;
+
+  modular_counter_namespace_subset :
+    ↑modular_counter_namespace ⊆ modular_counter_mask;
+
   modular_is_counter : modular_counter_name → val → iProp Σ;
+
   modular_handle : modular_counter_name → val → iProp Σ;
-  counter_model : modular_counter_name → Qp → nat → iProp Σ;
+
+  counter_auth : modular_counter_name → nat → iProp Σ;
+
+  counter_frag : modular_counter_name → Qp → nat → iProp Σ;
 
   modular_is_counter_persistent γ c ::
     Persistent (modular_is_counter γ c);
@@ -22,30 +34,30 @@ Class modular_counter (Σ : gFunctors) `{!heapGS Σ} := ModularCounter {
   modular_handle_persistent γ h ::
     Persistent (modular_handle γ h);
 
-  counter_model_fractional γ n ::
-    Fractional (λ q, counter_model γ q n);
+  counter_frag_fractional γ n ::
+    Fractional (λ q, counter_frag γ q n);
 
-  modular_new_counter_spec (E : coPset) (T : nat) :
-    ↑modular_counter_namespace ⊆ E →
+
+  modular_new_counter_spec (T : nat) :
     {{{ ⌜0 < T⌝ }}}
-      modular_new_counter #T @ E
+      modular_new_counter #T @ modular_counter_mask
     {{{ c γ, RET c;
         modular_is_counter γ c ∗
         ([∗ list] i ∈ seq 0 T,
           modular_handle γ #(i : nat)) ∗
-        counter_model γ (1 / 2)%Qp 0 }}};
+        counter_frag γ 1%Qp 0 }}};
+
 
   modular_incr_spec
-      (E : coPset) γ c h
+      γ c h
       (P : iProp Σ) (Q : nat → iProp Σ) :
-    ↑modular_counter_namespace ⊆ E →
     (∀ total,
-      □ (counter_model γ (1 / 2)%Qp total ∗ P
-          ={E ∖ ↑modular_counter_namespace}=∗
-         counter_model γ (1 / 2)%Qp (S total) ∗ Q total)) ⊢
+      □ (counter_auth γ total ∗ P
+          ={modular_counter_mask ∖ ↑modular_counter_namespace}=∗
+         counter_auth γ (S total) ∗ Q total)) ⊢
     {{{ modular_is_counter γ c ∗
         modular_handle γ h ∗ P }}}
-      modular_incr c h @ E
+      modular_incr c h @ modular_counter_mask
     {{{ RET #();
         modular_is_counter γ c ∗
         modular_handle γ h ∗
@@ -53,15 +65,14 @@ Class modular_counter (Σ : gFunctors) `{!heapGS Σ} := ModularCounter {
 
 
   modular_read_spec
-      (E : coPset) γ c
+      γ c
       (P : iProp Σ) (Q : nat → iProp Σ) :
-    ↑modular_counter_namespace ⊆ E →
     (∀ total,
-      □ (counter_model γ (1 / 2)%Qp total ∗ P
-          ={E ∖ ↑modular_counter_namespace}=∗
-         counter_model γ (1 / 2)%Qp total ∗ Q total)) ⊢
+      □ (counter_auth γ total ∗ P
+          ={modular_counter_mask ∖ ↑modular_counter_namespace}=∗
+         counter_auth γ total ∗ Q total)) ⊢
     {{{ modular_is_counter γ c ∗ P }}}
-      modular_read c @ E
+      modular_read c @ modular_counter_mask
     {{{ (total : nat), RET #total;
         modular_is_counter γ c ∗
         Q total }}};
