theories/sharded_counter_refinement.v
@@ -1,0 +1,640 @@
+From iris.algebra Require Import auth excl gmap.
+From iris.proofmode Require Import proofmode.
+From iris.heap_lang Require Import lang notation tactics.
+From reloc Require Import reloc.
+From reloc.lib Require Import counter lock.
+From reloc.logic Require Import spec_ra spec_rules.
+From summer_project Require Import sharded_counter_modular.
+
+Set Default Proof Using "Type".
+
+Definition msc_counter : val :=
+  λ: <>,
+    let: "c" := msc_new_counter #2 in
+    ((λ: "k", msc_incr "c" "k"),
+     (λ: <>, msc_read "c")).
+
+Definition msc_counter2 : val :=
+  λ: <>,
+    let: "c" := msc_counter #() in
+    (((λ: <>, (Fst "c") #0),
+      (λ: <>, (Fst "c") #1)),
+     Snd "c").
+
+Definition linear_counter2 : val :=
+  λ: <>,
+    let: "c" := FG_counter #() in
+    (((λ: <>, (Fst "c") #();; #()),
+      (λ: <>, (Fst "c") #();; #())),
+     Snd "c").
+
+Definition sequential_counter2 : val :=
+  λ: <>,
+    let: "c" := CG_counter #() in
+    (((λ: <>, (Fst "c") #();; #()),
+      (λ: <>, (Fst "c") #();; #())),
+     Snd "c").
+
+Definition counter2_type : type :=
+  TArrow TUnit
+    (TProd
+      (TProd (TArrow TUnit TUnit) (TArrow TUnit TUnit))
+      (TArrow TUnit TNat)).
+
+Section refinement.
+  Context `{!relocG Σ, !mscG Σ}.
+
+  Definition msc_refinementN : namespace := nroot .@ "msc_refinement".
+
+  Definition msc_linear_inv (γ : msc_name) (x : loc) : iProp Σ :=
+    (∃ n : nat, msc_frag γ 1%Qp n ∗ x ↦ₛ #n)%I.
+
+  Lemma lrel_pair_intro (A B : lrel Σ) v1 v2 v1' v2' :
+    A v1 v1' -∗
+    B v2 v2' -∗
+    (A * B)%lrel (v1, v2)%V (v1', v2')%V.
+  Proof.
+    iIntros "HA HB".
+    iExists v1, v1', v2, v2'.
+    iSplit; first done. iSplit; first done. iFrame.
+  Qed.
+
+  Lemma msc_linear_incr_refinement γ c h x :
+    msc_is_counter γ c -∗
+    msc_handle γ h -∗
+    inv msc_refinementN (msc_linear_inv γ x) -∗
+    REL msc_incr c h << (FG_increment #x;; #()) : ().
+  Proof.
+    iIntros "#Hcounter #Hhandle #Hinv".
+    rewrite refines_eq /refines_def.
+    iIntros (j) "Hj".
+    iModIntro.
+    wp_apply (msc_incr_spec γ c h
+      (refines_right j (FG_increment #x;; #()))%I
+      (λ _, refines_right j #())%I with "[] [$Hcounter $Hhandle $Hj]").
+    - iIntros (total) "!# [Hauth Hj]".
+      iInv msc_refinementN as (n) "[>Hfrag >Hx]" "Hclose".
+      iDestruct (msc_auth_frag_agree with "Hauth Hfrag") as %->.
+
+      iEval (rewrite /FG_increment) in "Hj".
+      tp_rec j. tp_pures j. tp_load j. tp_pures j.
+      tp_cmpxchg_suc j. tp_pures j.
+
+      iMod (msc_auth_frag_update γ n n (S n)
+        with "Hauth Hfrag") as "[Hauth Hfrag]".
+      iMod ("Hclose" with "[Hfrag Hx]") as "_".
+      { iNext. iExists (S n). iFrame.
+        rewrite Nat2Z.inj_succ Z.add_comm. iFrame. }
+      iModIntro. iFrame.
+    - iIntros "(#Hcounter' & #Hhandle' & Hdone)".
+      iDestruct "Hdone" as (total) "Hj".
+      iExists #(). iFrame "Hj".
+      iPureIntro. done.
+  Qed.
+
+  Lemma msc_linear_read_refinement γ c x :
+    msc_is_counter γ c -∗
+    inv msc_refinementN (msc_linear_inv γ x) -∗
+    REL msc_read c << counter_read #x : lrel_int.
+  Proof.
+    iIntros "#Hcounter #Hinv".
+    rewrite refines_eq /refines_def.
+    iIntros (j) "Hj".
+    iModIntro.
+    wp_apply (msc_read_spec γ c
+      (refines_right j (counter_read #x))%I
+      (λ total, refines_right j #(total : nat))%I
+      with "[] [$Hcounter $Hj]").
+    - iIntros (total) "!# [Hauth Hj]".
+      iInv msc_refinementN as (n) "[>Hfrag >Hx]" "Hclose".
+      iDestruct (msc_auth_frag_agree with "Hauth Hfrag") as %->.
+
+      iEval (rewrite /counter_read) in "Hj".
+      tp_rec j. tp_pures j. tp_load j. tp_pures j.
+
+      iMod ("Hclose" with "[Hfrag Hx]") as "_".
+      { iNext. iExists n. iFrame. }
+      iModIntro. iFrame.
+    - iIntros (total) "[#Hcounter' Hj]".
+      iExists #(total : nat). iFrame "Hj".
+      iExists (Z.of_nat total). iPureIntro. done.
+  Qed.
+
+  Lemma msc_linear_counter_refinement :
+    ⊢ REL msc_counter2 << linear_counter2 :
+        () → ((() → ()) * (() → ())) * (() → lrel_int).
+  Proof using Type*.
+    rewrite /msc_counter2 /linear_counter2 /msc_counter /FG_counter.
+    iApply refines_arrow_val.
+    iModIntro. iIntros (v1 v2) "Hunit".
+    iDestruct "Hunit" as %[-> ->].
+    rel_rec_l. rel_rec_r. rel_pures_r.
+    rel_alloc_r x as "Hx".
+    rel_pures_r.
+    rel_apply_l refines_wp_l. wp_pures.
+    wp_bind (msc_new_counter #2).
+    wp_apply (msc_new_counter_spec 2).
+    { iPureIntro. lia. }
+    iIntros (c γ) "(#Hcounter & Hhandles & Hfrag)".
+    iEval (rewrite /=) in "Hhandles".
+    iDestruct "Hhandles" as "(#Hhandle0 & #Hhandle1 & _)".
+
+    iMod (inv_alloc msc_refinementN _ (msc_linear_inv γ x)
+      with "[Hfrag Hx]") as "#Hinv".
+    { iNext. iExists 0. iFrame. }
+
+    wp_pures.
+    iModIntro.
+    iApply refines_ret. iModIntro.
+    iApply lrel_pair_intro.
+    - iApply lrel_pair_intro.
+      + iModIntro. iIntros (u1 u2) "Hunit".
+        iDestruct "Hunit" as %[-> ->].
+        rel_seq_l. rel_seq_r. rel_pures_l. rel_pures_r.
+        iApply (msc_linear_incr_refinement with "Hcounter Hhandle0 Hinv").
+      + iModIntro. iIntros (u1 u2) "Hunit".
+        iDestruct "Hunit" as %[-> ->].
+        rel_seq_l. rel_seq_r. rel_pures_l. rel_pures_r.
+        iApply (msc_linear_incr_refinement with "Hcounter Hhandle1 Hinv").
+    - iModIntro. iIntros (u1 u2) "Hunit".
+      iDestruct "Hunit" as %[-> ->].
+      rel_seq_l. rel_seq_r.
+      iApply (msc_linear_read_refinement with "Hcounter Hinv").
+  Qed.
+
+End refinement.
+
+Theorem msc_linear_ctx_refinement :
+  ∅ ⊨ msc_counter2 ≤ctx≤ linear_counter2 : counter2_type.
+Proof.
+  pose (Σ := #[relocΣ; mscΣ]).
+  eapply (refines_sound Σ).
+  iIntros (? Δ).
+  iApply msc_linear_counter_refinement.
+Qed.
+
+Section linear_sequential_refinement.
+  Context `{!relocG Σ}.
+
+  Lemma linear_sequential_counter_refinement :
+    ⊢ REL linear_counter2 << sequential_counter2 :
+        () → ((() → ()) * (() → ())) * (() → lrel_int).
+  Proof using Type*.
+    rewrite /linear_counter2 /sequential_counter2 /FG_counter /CG_counter.
+    iApply refines_arrow_val.
+    iModIntro. iIntros (v1 v2) "Hunit".
+    iDestruct "Hunit" as %[-> ->].
+    rel_rec_l. rel_rec_r. rel_pures_r.
+    rel_apply_r refines_newlock_r; auto.
+    iIntros (lk) "Hlk".
+    repeat rel_pure_r.
+    rel_alloc_r cnt' as "Hcnt'".
+    rel_pures_l. rel_alloc_l cnt as "Hcnt".
+
+    iAssert (counter_inv lk cnt cnt') with "[Hlk Hcnt Hcnt']" as "Hinv".
+    { iExists 0. by iFrame. }
+    iMod (inv_alloc counterN with "[Hinv]") as "#Hinv".
+    { iNext. iExact "Hinv". }
+
+    rel_pures_r. rel_pures_l.
+    iApply refines_ret. iModIntro.
+    iApply lrel_pair_intro.
+    - iApply lrel_pair_intro.
+      + iModIntro. iIntros (u1 u2) "Hunit".
+        iDestruct "Hunit" as %[-> ->].
+        rel_seq_l. rel_seq_r. rel_pures_l. rel_pures_r.
+        iApply (refines_seq lrel_int).
+        * iApply (FG_CG_increment_refinement with "Hinv").
+        * rel_values.
+      + iModIntro. iIntros (u1 u2) "Hunit".
+        iDestruct "Hunit" as %[-> ->].
+        rel_seq_l. rel_seq_r. rel_pures_l. rel_pures_r.
+        iApply (refines_seq lrel_int).
+        * iApply (FG_CG_increment_refinement with "Hinv").
+        * rel_values.
+    - iModIntro. iIntros (u1 u2) "Hunit".
+      iDestruct "Hunit" as %[-> ->]. rel_seq_l. rel_seq_r. iApply (counter_read_refinement with "Hinv").
+  Qed.
+
+End linear_sequential_refinement.
+
+
+Theorem linear_sequential_ctx_refinement :
+  ∅ ⊨ linear_counter2 ≤ctx≤ sequential_counter2 : counter2_type.
+Proof.
+  eapply (refines_sound relocΣ).
+  iIntros (? Δ).
+  iApply linear_sequential_counter_refinement.
+Qed.
+
+Theorem msc_sequential_ctx_refinement :
+  ∅ ⊨ msc_counter2 ≤ctx≤ sequential_counter2 : counter2_type.
+Proof.
+  eapply (ctx_refines_transitive ∅ counter2_type
+    msc_counter2 linear_counter2 sequential_counter2).
+  - exact msc_linear_ctx_refinement.
+  - exact linear_sequential_ctx_refinement.
+Qed.
+
+(** ReLoC only exposes a right-hand rule for one-cell allocation.  The
+    sharded wrapper allocates exactly two consecutive cells, so the reverse
+    refinement needs the corresponding specification-side rule. *)
+Section spec_alloc2.
+  Context `{!relocG Σ}.
+
+  Lemma step_alloc2 E j K (v : val) :
+    nclose specN ⊆ E →
+    spec_ctx ∗ j ⤇ fill K (AllocN #2 (of_val v)) ={E}=∗
+      ∃ l : loc, spec_ctx ∗ j ⤇ fill K (#l) ∗
+           l ↦ₛ v ∗ (l +ₗ 1) ↦ₛ v.
+  Proof.
+    iIntros (HE) "[#Hspec Hj]".
+    iFrame "Hspec".
+    rewrite /spec_ctx tpool_pointsto_eq /tpool_pointsto_def /=.
+    iDestruct "Hspec" as (ρ) "Hspec".
+    iInv specN as (tp σ) ">[Hown %Hsteps]" "Hclose".
+    pose (l := Loc.fresh (dom (heap σ))).
+    pose (ins0 := λ h : gmap loc (option val), <[l:=Some v]> h).
+    pose (ins1 := λ h : gmap loc (option val), <[l +ₗ 1:=Some v]> h).
+    iCombine "Hown Hj"
+      gives %[[Htp%tpool_singleton_included' _]%prod_included
+               _]%auth_both_valid_discrete.
+    pose proof (tpool_lookup_Some tp j
+      (fill K (AllocN #2 (of_val v))) Htp) as Htp'.
+    iMod (own_update_2 with "Hown Hj") as "[Hown Hj]".
+    { by eapply auth_update, prod_local_update_1,
+        singleton_local_update,
+        (exclusive_local_update _ (Excl (fill K (#l)%E))). }
+    iMod (own_update with "Hown") as "[Hown Hl1]".
+    { eapply auth_update_alloc, prod_local_update_2, prod_local_update_2,
+        (alloc_singleton_local_update _ (l +ₗ 1)
+          (1%Qp, to_agree (Some v : leibnizO _))); last done.
+      apply lookup_to_heap_None.
+      apply not_elem_of_dom_1.
+      unfold l.
+      apply Loc.fresh_fresh. lia. }
+    iMod (own_update with "Hown") as "[Hown Hl0]".
+    { eapply auth_update_alloc, prod_local_update_2, prod_local_update_2,
+        (alloc_singleton_local_update _ l
+          (1%Qp, to_agree (Some v : leibnizO _))); last done.
+      rewrite lookup_insert_ne.
+      - apply lookup_to_heap_None.
+        apply not_elem_of_dom_1.
+        unfold l.
+        rewrite -{1}(Loc.add_0 (Loc.fresh (dom (heap σ)))).
+        apply Loc.fresh_fresh. lia.
+      - intros Heq. apply Loc.eq_spec in Heq. simpl in Heq. lia. }
+    rewrite !heapS_pointsto_eq /heapS_pointsto_def /=.
+    iExists l. iFrame "Hj Hl0 Hl1".
+    iApply "Hclose". iNext.
+    iExists (<[j:=fill K (#l)]> tp),
+      (state_upd_heap ins0 (state_upd_heap ins1 σ)).
+    rewrite /to_state !to_heap_insert to_tpool_insert'; last eauto.
+    iFrame "Hown".
+    iPureIntro.
+    eapply rtc_r.
+    - exact Hsteps.
+    - eapply step_insert_no_fork.
+      + exact Htp'.
+      + replace
+          (state_upd_heap ins0 (state_upd_heap ins1 σ))
+          with (state_init_heap l 2 v σ).
+        * apply alloc_fresh. lia.
+        * destruct σ as [h ps]. unfold ins0, ins1.
+          rewrite /state_init_heap /= /heap_array /=.
+          f_equal. rewrite -assoc_L.
+          rewrite right_id. by rewrite !insert_union_singleton_l.
+  Qed.
+
+  Lemma refines_alloc2_r E (K : list ectx_item) (t : expr)
+      (v : val) (A : lrel Σ) :
+    nclose specN ⊆ E →
+    (∀ l, l ↦ₛ v -∗ (l +ₗ 1) ↦ₛ v -∗
+      REL t << fill K (#l) @ E : A) -∗
+    REL t << fill K (AllocN #2 (of_val v)) @ E : A.
+  Proof.
+    iIntros (HE) "Hcont".
+    iApply refines_step_r.
+    iIntros (j) "Hj".
+    iMod (step_alloc2 with "Hj") as (l) "($ & Hj & Hl0 & Hl1)"; first done.
+    iModIntro. iExists #l. iFrame "Hj".
+    iApply ("Hcont" with "Hl0 Hl1").
+  Qed.
+End spec_alloc2.
+
+Section linear_msc_reverse.
+  Context `{!relocG Σ}.
+
+  Definition linear_msc_reverseN : namespace :=
+    nroot .@ "linear_msc_reverse".
+
+  Definition linear_msc_reverse_inv (x a : loc) : iProp Σ :=
+    (∃ n0 n1 : nat,
+      x ↦ #((n0 + n1)%nat) ∗ a ↦ₛ #n0 ∗ (a +ₗ 1) ↦ₛ #n1)%I.
+
+  Definition linear_msc_reverse_state (a : loc) (n : nat) : iProp Σ :=
+    (∃ n0 n1 : nat,
+      ⌜n = (n0 + n1)%nat⌝ ∗ a ↦ₛ #n0 ∗ (a +ₗ 1) ↦ₛ #n1)%I.
+
+  Lemma linear_msc_incr0_refinement x a :
+    inv linear_msc_reverseN (linear_msc_reverse_inv x a) -∗
+    REL (FG_increment #x;; #()) << msc_incr (#a, #2)%V #0 : ().
+  Proof.
+    iIntros "#Hinv".
+    rel_apply_l
+      (FG_increment_atomic_l (linear_msc_reverse_state a) True%I);
+      first done.
+    iModIntro.
+    iInv linear_msc_reverseN as (n0 n1) "(>Hx & >Ha0 & >Ha1)" "Hclose".
+    iModIntro.
+    iExists (n0 + n1)%nat. iFrame "Hx".
+    iSplitL "Ha0 Ha1".
+    { iExists n0, n1. iFrame. done. }
+    iSplit.
+    - iIntros "(Hx & Hstate)".
+      iDestruct "Hstate" as (m0 m1 ->) "(Ha0 & Ha1)".
+      iApply "Hclose". iNext. iExists m0, m1. iFrame.
+    - iIntros "(Hx & Hstate) _".
+      iDestruct "Hstate" as (m0 m1 ->) "(Ha0 & Ha1)".
+      rewrite /msc_incr.
+      rel_pures_r. rewrite Loc.add_0.
+      rel_apply_r (refines_faa_r _ _ _ _ (Z.of_nat m0) 1 _ _ with "Ha0").
+      iIntros "Ha0".
+      iMod ("Hclose" with "[Hx Ha0 Ha1]") as "_".
+      { iNext. iExists (m0 + 1)%nat, m1.
+        replace (m0 + 1 + m1)%nat with (m0 + m1 + 1)%nat by lia.
+        rewrite !Nat2Z.inj_add /=.
+        iFrame. }
+      rel_pures_r. rel_pures_l. rel_values.
+  Qed.
+
+  Lemma linear_msc_incr1_refinement x a :
+    inv linear_msc_reverseN (linear_msc_reverse_inv x a) -∗
+    REL (FG_increment #x;; #()) << msc_incr (#a, #2)%V #1 : ().
+  Proof.
+    iIntros "#Hinv".
+    rel_apply_l
+      (FG_increment_atomic_l (linear_msc_reverse_state a) True%I);
+      first done.
+    iModIntro.
+    iInv linear_msc_reverseN as (n0 n1) "(>Hx & >Ha0 & >Ha1)" "Hclose".
+    iModIntro.
+    iExists (n0 + n1)%nat. iFrame "Hx".
+    iSplitL "Ha0 Ha1".
+    { iExists n0, n1. iFrame. done. }
+    iSplit.
+    - iIntros "(Hx & Hstate)".
+      iDestruct "Hstate" as (m0 m1 ->) "(Ha0 & Ha1)".
+      iApply "Hclose". iNext. iExists m0, m1. iFrame.
+    - iIntros "(Hx & Hstate) _".
+      iDestruct "Hstate" as (m0 m1 ->) "(Ha0 & Ha1)".
+      rewrite /msc_incr.
+      rel_pures_r.
+      rel_apply_r (refines_faa_r _ _ _ _ (Z.of_nat m1) 1 _ _ with "Ha1").
+      iIntros "Ha1".
+      iMod ("Hclose" with "[Hx Ha0 Ha1]") as "_".
+      { iNext. iExists m0, (m1 + 1)%nat.
+        replace (m0 + (m1 + 1))%nat with (m0 + m1 + 1)%nat by lia. rewrite !Nat2Z.inj_add /=.
+        iFrame. }
+      rel_pures_r. rel_pures_l. rel_values.
+  Qed.
+
+  Lemma linear_msc_read_refinement x a :
+    inv linear_msc_reverseN (linear_msc_reverse_inv x a) -∗
+    REL counter_read #x << msc_read (#a, #2)%V : lrel_int.
+  Proof.
+    iIntros "#Hinv".
+    rel_apply_l
+      (counter_read_atomic_l (linear_msc_reverse_state a) True%I);
+      first done.
+    iModIntro.
+    iInv linear_msc_reverseN as (n0 n1) "(>Hx & >Ha0 & >Ha1)" "Hclose".
+    iModIntro.
+    iExists (n0 + n1)%nat. iFrame "Hx".
+    iSplitL "Ha0 Ha1".
+    { iExists n0, n1. iFrame. done. }
+    iSplit.
+    - iIntros "(Hx & Hstate)".
+      iDestruct "Hstate" as (m0 m1 ->) "(Ha0 & Ha1)".
+      iApply "Hclose". iNext. iExists m0, m1. iFrame.
+    - iIntros "(Hx & Hstate) _".
+      iDestruct "Hstate" as (m0 m1 ->) "(Ha0 & Ha1)".
+      rewrite /msc_read.
+      rel_pures_r.
+      rel_newproph_r p as "#Hp".
+      rel_pures_r. rewrite /msc_sum_loop. rel_pures_r. rewrite Loc.add_0. rel_load_r. rel_pures_r. rel_load_r. rel_pures_r.
+      iMod ("Hclose" with "[Hx Ha0 Ha1]") as "_".
+      { iNext. iExists m0, m1. iFrame. }
+      rel_resolveproph_r.
+      rel_pures_r.
+      rel_values.
+      iExists (Z.of_nat (m0 + m1)). iPureIntro. split; first done. f_equal; try reflexivity. rewrite Nat2Z.inj_add. simpl. reflexivity.
+  Qed.
+
+  Lemma linear_msc_counter_refinement :
+    ⊢ REL linear_counter2 << msc_counter2 :
+        () → ((() → ()) * (() → ())) * (() → lrel_int).
+  Proof using Type*.
+    rewrite /linear_counter2 /msc_counter2 /FG_counter /msc_counter.
+    iApply refines_arrow_val.
+    iModIntro. iIntros (v1 v2) "Hunit".
+    iDestruct "Hunit" as %[-> ->].
+    rel_rec_l. rel_rec_r. rel_pures_l. rel_pures_r.
+    rel_alloc_l x as "Hx".
+    rel_pures_l.
+    rewrite /msc_new_counter.
+    rel_pures_r.
+    rel_apply_r refines_alloc2_r; first auto.
+    iIntros (a) "Ha0 Ha1".
+    rel_pures_r.
+    iMod (inv_alloc linear_msc_reverseN _ (linear_msc_reverse_inv x a)
+      with "[Hx Ha0 Ha1]") as "#Hinv".
+    { iNext. iExists 0%nat, 0%nat. iFrame. }
+    iApply refines_ret. iModIntro.
+    iApply lrel_pair_intro.
+    - iApply lrel_pair_intro.
+      + iModIntro. iIntros (u1 u2) "Hunit".
+        iDestruct "Hunit" as %[-> ->].
+        rel_seq_l. rel_seq_r. rel_pures_l. rel_pures_r.
+        iApply (linear_msc_incr0_refinement with "Hinv").
+      + iModIntro. iIntros (u1 u2) "Hunit".
+        iDestruct "Hunit" as %[-> ->].
+        rel_seq_l. rel_seq_r. rel_pures_l. rel_pures_r.
+        iApply (linear_msc_incr1_refinement with "Hinv").
+    - iModIntro. iIntros (u1 u2) "Hunit".
+      iDestruct "Hunit" as %[-> ->].
+      rel_seq_l. rel_seq_r.
+      iApply (linear_msc_read_refinement with "Hinv").
+  Qed.
+End linear_msc_reverse.
+
+Theorem linear_msc_ctx_refinement :
+  ∅ ⊨ linear_counter2 ≤ctx≤ msc_counter2 : counter2_type.
+Proof.
+  eapply (refines_sound relocΣ).
+  iIntros (? Δ).
+  iApply linear_msc_counter_refinement.
+Qed.
+
+Section sequential_linear_reverse.
+  Context `{!relocG Σ, !lockG Σ}.
+
+  Definition sequential_linear_lockN : namespace :=
+    nroot .@ "sequential_linear_lock".
+  Definition sequential_linear_counterN : namespace :=
+    nroot .@ "sequential_linear_counter".
+
+  Definition sequential_linear_lock_res (x : loc) : iProp Σ :=
+    (∃ z : Z, x ↦{#1/2} #z)%I.
+
+  Definition sequential_linear_inv (x y : loc) : iProp Σ :=
+    (∃ z : Z, x ↦{#1/2} #z ∗ y ↦ₛ #z)%I.
+
+  Lemma FG_increment_Z_r K E t A (y : loc) (z : Z) :
+    nclose specN ⊆ E →
+    y ↦ₛ #z -∗
+    (y ↦ₛ #(1 + z) -∗
+      REL t << fill K (of_val #z) @ E : A) -∗
+    REL t << fill K (FG_increment #y) @ E : A.
+  Proof.
+    iIntros (?) "Hy Hcont".
+    rewrite /FG_increment.
+    rel_rec_r. repeat rel_pure_r.
+    rel_load_r. repeat rel_pure_r.
+    rel_cmpxchg_suc_r. rel_pures_r.
+    by iApply ("Hcont" with "Hy").
+  Qed.
+
+  Lemma sequential_linear_incr_refinement γ lk x y :
+    is_lock sequential_linear_lockN γ #lk (sequential_linear_lock_res x) -∗
+    inv sequential_linear_counterN (sequential_linear_inv x y) -∗
+    REL (CG_increment #x #lk;; #()) << (FG_increment #y;; #()) : ().
+  Proof.
+    iIntros "#Hlock #Hinv".
+    rewrite /CG_increment.
+    rel_pures_l.
+    rel_apply_l (refines_acquire_l sequential_linear_lockN
+      (sequential_linear_lock_res x) with "Hlock").
+    iNext. iIntros "Hlocked Hres".
+    iDestruct "Hres" as (n) "Hx".
+    rel_pures_l. rel_load_l. rel_pures_l.
+    rel_store_l_atomic.
+    iInv sequential_linear_counterN as (m) "(>Hx' & >Hy)" "Hclose".
+    iDestruct (pointsto_agree with "Hx Hx'") as %Heq.
+    simplify_eq.
+    iCombine "Hx Hx'" as "Hx".
+    iModIntro. iExists _. iFrame "Hx". iNext.
+    iIntros "Hx".
+    rel_apply_r (FG_increment_Z_r with "Hy").
+    iIntros "Hy".
+    iDestruct "Hx" as "[Hx Hx']".
+    iMod ("Hclose" with "[Hx' Hy]") as "_".
+    { iNext. iExists (1 + m)%Z. iFrame. }
+    rel_pures_l.
+    rel_apply_l (refines_release_l sequential_linear_lockN
+      (sequential_linear_lock_res x) with "Hlock Hlocked [Hx]").
+    { iExists (1 + m)%Z. iFrame. }
+    iNext.
+    rel_pures_l. rel_pures_r. rel_values.
+  Qed.
+
+  Lemma sequential_linear_read_refinement x y :
+    inv sequential_linear_counterN (sequential_linear_inv x y) -∗
+    REL counter_read #x << counter_read #y : lrel_int.
+  Proof.
+    iIntros "#Hinv".
+    rewrite /counter_read.
+    rel_pures_l.
+    rel_load_l_atomic.
+    iInv sequential_linear_counterN as (z) "(>Hx & >Hy)" "Hclose".
+    iModIntro. iExists #z. iFrame "Hx". iNext.
+    iIntros "Hx".
+    rel_load_r.
+    iMod ("Hclose" with "[Hx Hy]") as "_".
+    { iNext. iExists z. iFrame. }
+    rel_values.
+
+  Qed.
+
+  Lemma sequential_linear_counter_refinement :
+    ⊢ REL sequential_counter2 << linear_counter2 :
+        () → ((() → ()) * (() → ())) * (() → lrel_int).
+  Proof using Type*.
+    rewrite /sequential_counter2 /linear_counter2 /CG_counter /FG_counter.
+    iApply refines_arrow_val.
+    iModIntro. iIntros (v1 v2) "Hunit".
+    iDestruct "Hunit" as %[-> ->].
+    rel_rec_l. rel_rec_r. rewrite /newlock. rel_pures_l. rel_pures_r.
+
+    rel_pures_l. rel_alloc_l lk as "Hlk". rel_pures_l. rel_alloc_l x as "Hx". rel_pures_l. rel_alloc_r y as "Hy". rel_pures_r.
+    iDestruct "Hx" as "[HxL HxG]".
+    iMod (own_alloc (Excl ())) as (γ) "Hγ"; first done.
+    iMod (inv_alloc sequential_linear_lockN _
+      (lock_inv γ lk (sequential_linear_lock_res x))
+      with "[Hlk Hγ HxL]") as "#Hlock_inv".
+    { iNext. iExists false. iFrame. }
+    iAssert (is_lock sequential_linear_lockN γ #lk
+      (sequential_linear_lock_res x)) as "#Hlock".
+    { iExists lk. iSplit; first done. iExact "Hlock_inv". }
+    iMod (inv_alloc sequential_linear_counterN _
+      (sequential_linear_inv x y) with "[HxG Hy]") as "#Hinv".
+    { iNext. iExists 0%Z. iFrame. }
+    iApply refines_ret. iModIntro.
+    iApply lrel_pair_intro.
+    - iApply lrel_pair_intro.
+      + iModIntro. iIntros (u1 u2) "Hunit".
+        iDestruct "Hunit" as %[-> ->].
+        rel_seq_l. rel_seq_r. rel_pures_l. rel_pures_r.
+        iApply (sequential_linear_incr_refinement with "Hlock Hinv").
+      + iModIntro. iIntros (u1 u2) "Hunit".
+        iDestruct "Hunit" as %[-> ->].
+        rel_seq_l. rel_seq_r. rel_pures_l. rel_pures_r.
+        iApply (sequential_linear_incr_refinement with "Hlock Hinv").
+    - iModIntro. iIntros (u1 u2) "Hunit".
+      iDestruct "Hunit" as %[-> ->].
+      rel_seq_l. rel_seq_r.
+      iApply (sequential_linear_read_refinement with "Hinv").
+  Qed.
+End sequential_linear_reverse.
+
+Theorem sequential_linear_ctx_refinement :
+  ∅ ⊨ sequential_counter2 ≤ctx≤ linear_counter2 : counter2_type.
+Proof.
+  pose (Σ := #[relocΣ; lockΣ]).
+  eapply (refines_sound Σ).
+  iIntros (? Δ).
+  iApply sequential_linear_counter_refinement.
+Qed.
+
+Theorem sequential_msc_ctx_refinement :
+  ∅ ⊨ sequential_counter2 ≤ctx≤ msc_counter2 : counter2_type.
+Proof.
+  eapply (ctx_refines_transitive ∅ counter2_type
+    sequential_counter2 linear_counter2 msc_counter2).
+  - exact sequential_linear_ctx_refinement.
+  - exact linear_msc_ctx_refinement.
+Qed.
+
+Theorem msc_linear_ctx_equiv :
+  ∅ ⊨ msc_counter2 =ctx= linear_counter2 : counter2_type.
+Proof.
+  split.
+  - exact msc_linear_ctx_refinement.
+  - exact linear_msc_ctx_refinement.
+Qed.
+
+Theorem linear_sequential_ctx_equiv :
+  ∅ ⊨ linear_counter2 =ctx= sequential_counter2 : counter2_type.
+Proof.
+  split.
+  - exact linear_sequential_ctx_refinement.
+  - exact sequential_linear_ctx_refinement.
+Qed.
+
+Theorem msc_sequential_ctx_equiv :
+  ∅ ⊨ msc_counter2 =ctx= sequential_counter2 : counter2_type.
+Proof.
+  split.
+  - exact msc_sequential_ctx_refinement.
+  - exact sequential_msc_ctx_refinement.
+Qed.
